SystemFD/Metatheory/Inversion.lean
@@ -1,0 +1,42 @@
+import SystemFD.Term
+import SystemFD.Judgment
+import SystemFD.Ctx
+
+theorem inversion_apply_spine :
+  Γ ⊢ t.apply_spine sp : A ->
+  ∃ B, Γ ⊢ t : B
+:= by
+intro j; induction sp generalizing Γ t A <;> simp at *
+case _ => exists A
+case _ hd tl ih =>
+  cases hd; case _ v a =>
+  cases v <;> simp at *
+  case _ =>
+    replace ih := ih j
+    cases ih; case _ B ih =>
+    cases ih; case _ j1 j2 j3 =>
+    apply Exists.intro _; apply j1
+  case _ =>
+    replace ih := ih j
+    cases ih; case _ B ih =>
+    cases ih; case _ j1 j2 j3 =>
+    apply Exists.intro _; apply j1
+  case _ =>
+    replace ih := ih j
+    cases ih; case _ B ih =>
+    cases ih; case _ j =>
+    apply Exists.intro _; apply j
+
+theorem ctx_get_term_well_typed :
+  ⊢ Γ ->
+  Γ d@ x = .term T t ->
+  Γ ⊢ t : T
+:= by sorry
+
+theorem ctx_get_instance_well_typed :
+  ⊢ Γ ->
+  Γ d@ x = .openm T ->
+  ixs = instance_indices' Γ 0 x [] ->
+  t ∈ get_instances Γ ixs ->
+  Γ ⊢ t : T
+:= by sorry
