SystemFD/Util.lean
@@ -5,6 +5,20 @@ def prefix_equal [BEq T] : List T -> List T -> Option (List T)
 | .cons _ _, [] => .none
 | .cons x1 t1, .cons x2 t2 => if x1 == x2 then prefix_equal t1 t2 else .none
 
+theorem prefix_equal_law [BEq T] [LawfulBEq T] {p t1 t2 : List T}
+  : .some p = prefix_equal t1 t2 -> t2 = t1 ++ p
+:= by
+intro h
+induction t1, t2 using prefix_equal.induct generalizing p
+case _ => simp at h; subst h; simp
+case _ => simp at h
+case _ h2 ih =>
+    replace h2 := LawfulBEq.eq_of_beq h2; subst h2
+    simp at h; rw [ih h]; simp
+case _ h2 =>
+  simp at *; exfalso
+  apply h2; apply h.1
+
 instance : Monad List where
   pure a := List.cons a List.nil
   bind l f := List.flatMap l f
